@prefix : <http://purl.org/ldht/> .
@prefix owl: <http://www.w3.org/2002/07/owl#> .
@prefix rdf: <http://www.w3.org/1999/02/22-rdf-syntax-ns#> .
@prefix xml: <http://www.w3.org/XML/1998/namespace> .
@prefix xsd: <http://www.w3.org/2001/XMLSchema#> .
@prefix rdfs: <http://www.w3.org/2000/01/rdf-schema#> .
@prefix schema: <http://schema.org/> .
@base <http://purl.org/ldht/> .

<http://purl.org/ldht/> rdf:type owl:Ontology ;
                         owl:versionIRI <http://purl.org/ldht/1.0/> ;
                         owl:imports <http://schema.org/> ,
                                     <https://w3id.org/tree#Ontology> ;
                         <http://purl.org/dc/terms/abstract> ""@en ;
                         <http://purl.org/dc/terms/bibliographicCitation> "Maxim Van de Wynckel, LDHT: A Distributed Linked Data Hash Tree" ;
                         <http://purl.org/dc/terms/contributor> "Beat Signer"@en ;
                         <http://purl.org/dc/terms/creator> "Maxim Van de Wynckel"@en ;
                         <http://purl.org/dc/terms/description> ""@en ;
                         <http://purl.org/dc/terms/license> <http://purl.org/NET/rdflicense/MIT1.0> ;
                         <http://purl.org/dc/terms/modified> "2024-09-24T00:00:00"^^xsd:dateTime ;
                         <http://purl.org/dc/terms/title> "Linked Data Hash Tree"@en ;
                         <http://purl.org/vocab/vann/preferredNamespacePrefix> "ldth" ;
                         <http://purl.org/vocab/vann/preferredNamespaceUri> "http://purl.org/ldht/"^^xsd:anyURI .

#################################################################
#    Data properties
#################################################################

###  http://purl.org/ldht/nodeID
:nodeID rdf:type owl:DatatypeProperty ;
        rdfs:domain :Node ;
        rdfs:range xsd:integer ;
        rdfs:comment "The node identifier is a number generated by using the hash algorithm of the network."@en ;
        rdfs:label "node identifier"@en .


###  http://purl.org/ldht/timeout
:timeout rdf:type owl:DatatypeProperty ;
         rdfs:domain schema:Action ;
         rdfs:range xsd:integer ;
         rdfs:comment "The timeout is the time in milliseconds that a node will wait for a response from another node."@en ;
         rdfs:label "timeout"@en .


#################################################################
#    Classes
#################################################################

###  http://purl.org/ldht/AddNodeAction
:AddNodeAction rdf:type owl:Class ;
               rdfs:subClassOf schema:AddAction ;
               rdfs:comment "The act of indicating to a node that a new node has joined the network."@en ;
               rdfs:label "Add node action"@en .


###  http://purl.org/ldht/Node
:Node rdf:type owl:Class ;
      rdfs:subClassOf <https://w3id.org/tree#Node> ;
      rdfs:comment "A dht:Node is a node in a distributed hash tree that may contain relations to other nodes in the distributed hash tree."@en ;
      rdfs:label "Node"@en .


###  http://purl.org/ldht/PingAction
:PingAction rdf:type owl:Class ;
            rdfs:subClassOf <http://org.semanticweb.owlapi/error#Error1> ,
                            schema:Action ;
            rdfs:comment "The act of pinging a node to request if it is still active and responding to actions."@en ;
            rdfs:label "Ping action"@en .


###  http://purl.org/ldht/RemoveNodeAction
:RemoveNodeAction rdf:type owl:Class ;
                  rdfs:subClassOf schema:DeleteAction ;
                  rdfs:comment "The act of indicating to a node that another node is removed in the network."@en ;
                  rdfs:label "Remove node action"@en .


###  http://purl.org/ldht/StoreValueAction
:StoreValueAction rdf:type owl:Class ;
                  rdfs:subClassOf schema:InsertAction ;
                  rdfs:comment "The act of storing a value in a node."@en ;
                  rdfs:label "Store value action"@en .

